operations/Linearize_scratch.thy
@@ -1,0 +1,468 @@
+theory Linearize_scratch                                                      
+  imports "Binders.MRBNF_Composition" "Binders.MRBNF_Recursor" 
+    "HOL-Library.FSet" "HOL-Library.Uprod"
+  keywords "linearize_mrbnf" :: thy_goal
+begin
+
+section "setup"
+
+ML_file "../Tools/mrbnf_linearize_tactics.ML"
+ML_file "../Tools/mrbnf_linearize.ML"
+
+
+declare [[bnf_internals]]
+declare [[mrbnf_internals]]
+declare [[typedef_overloaded]]
+declare [[ML_print_depth=1000]]
+
+section "binder_datatypes & errors"
+binder_datatype 'var lterm = Vr 'var | Ap "'var lterm" "'var lterm"
+  | Lm x::'var t::"'var lterm" binds x in t
+
+
+binder_datatype ('a, 'b::var) test = V 'b | B "'a set" | C x::'b t::"('a, 'b) test" binds x in t
+
+(*ML \<open>BNF_Util.permute_like_unique (op =) [0, 1] [0, ~1, ~1, 1, ~1] [Bound 4, Bound 3, Bound 2, Bound 1, Bound 0]\<close>*)
+
+
+print_mrbnfs
+
+section "MRBNF fun"
+definition domain :: "('a \<Rightarrow> 'b) \<Rightarrow> 'a set" where
+  "domain _ = UNIV"
+
+definition map_fun' :: "('a \<Rightarrow> 'a) \<Rightarrow> ('b \<Rightarrow> 'b') \<Rightarrow> ('a \<Rightarrow> 'b) \<Rightarrow> ('a \<Rightarrow> 'b')" where
+  "map_fun' d r f = r o f o (inv d)"
+
+abbreviation "rel_fun' \<equiv> rel_fun (=)"
+
+lemma map_fun'_id_comp: "map_fun' id f F = f o F"
+  apply (unfold map_fun'_def inv_id o_id)
+  by (rule refl)
+
+lemma range_map: "bij f \<Longrightarrow> range (map_fun' f g x) = g ` range x"
+  apply (unfold o_apply map_fun'_def)
+  apply (subst fun.set_map[THEN sym])
+  apply (auto)
+  by (metis inv_simp1 range_eqI)
+  
+lemma f_o_map_fun': "f o map_fun' g id F = map_fun' g f F"
+  apply (unfold map_fun'_def)
+  apply (unfold o_assoc id_o)
+  by (rule refl)
+
+lemma map_fun'_o_f: "map_fun' g id (f o F) = map_fun' g f F"
+  apply (unfold map_fun'_def)
+  apply (unfold o_assoc id_o)
+  by (rule refl)
+
+mrbnf "('a::var) \<Rightarrow> 'b"
+  map: map_fun'
+  sets: 
+    bound: domain live: range
+  bd: "natLeq" (* natLeq +c card_suc |UNIV| *)
+  rel: "rel_fun'"
+  subgoal 
+    apply (unfold map_fun'_def o_apply inv_id)
+    by (auto)
+  subgoal for f1 g1 f2 g2
+    apply (unfold map_fun'_def)
+    apply (subst o_inv_distrib; (assumption)?)
+    apply (unfold o_apply)
+    by (auto)
+  subgoal for F f1 g1 f2 g2
+    apply (unfold domain_def map_fun'_def image_def)
+    apply (simp)
+    apply (drule ext)
+    apply (unfold o_apply)
+    apply (rule ext)
+    apply (hypsubst_thin)
+    apply (rule fun_cong[of "(\<lambda>a. g1 (F a))" "(\<lambda>a. g2 (F a))"])
+    by (auto)
+  subgoal for f g
+    apply (unfold o_apply domain_def image_def)
+    by (auto simp add: bij_betw_imp_surj full_SetCompr_eq)
+  subgoal for f g
+    apply (rule ext)
+    by (simp add: range_map)
+  subgoal 
+    by (rule infinite_regular_card_order_natLeq)
+      (* fun_bd*)
+  subgoal for F
+    (*apply (unfold domain_def)
+    by (rule ordLess_bd_fun)*)
+    sorry
+  subgoal for F
+    (* by (rule fun.set_bd) *)
+    sorry
+  subgoal for R S
+    by (simp add: fun.rel_compp)
+  subgoal for f R F G
+    apply (unfold fun.in_rel mem_Collect_eq map_fun'_id_comp)
+    apply (intro iffI)
+     apply (elim conjE exE)
+    subgoal premises prems for Z
+      apply (intro exI[of _ "(map_fun' (inv f) id) Z"] conjI)
+        apply (unfold range_map[OF bij_imp_bij_inv[OF prems(1)], of id Z] image_id f_o_map_fun')
+        apply (rule prems)
+       apply (unfold f_o_map_fun' arg_cong[OF prems(4), of "map_fun' (inv f) id", unfolded map_fun'_o_f])
+       apply (unfold map_fun'_def o_assoc id_o inv_inv_eq[OF prems(1)])[]
+       apply (auto simp add: prems(1))
+      apply (unfold map_fun'_def o_assoc inv_inv_eq[OF prems(1)])
+      apply (subst (3) o_assoc[THEN sym])
+      apply (unfold inv_o_simp2[OF prems(1)] o_id)
+      apply (rule prems)
+      done
+    apply (elim conjE exE)
+    subgoal premises prems for Z
+      apply (intro exI[of _ "(map_fun' f id) Z"] conjI)
+        apply (unfold range_map[OF prems(1), of id Z] image_id)
+        apply (rule prems)
+       apply (unfold f_o_map_fun' arg_cong[OF prems(4), of "map_fun' f id", unfolded map_fun'_o_f])
+       apply (rule refl)
+      apply (rule prems)
+      done
+    done
+  done
+
+section "Intuition: What is nonrep?"
+
+(* LIST *)
+lemma "\<And> R (x :: 'a list) y. list_all2 R x y = (\<exists>z. set z \<subseteq> {(x, y). R x y} \<and> map fst z = x \<and> map snd z = y)"
+  subgoal for R x y
+    apply (rule list.in_rel[of R x y, unfolded mem_Collect_eq])
+    done
+  done
+
+definition eq_shape_list :: "'a list \<Rightarrow> 'a list \<Rightarrow> bool" where 
+  "eq_shape_list x x' \<equiv> list_all2 top x x'"
+
+definition nonrep_list :: "'a list \<Rightarrow> bool" where 
+  "nonrep_list x \<equiv> \<forall> x'. eq_shape_list x x' \<longrightarrow> (\<exists> f. x' = map f x)"
+
+lemma eq_shape_list_alt: "list_all2 top xs xs' = (length xs = length xs')"
+  by (simp add: list_all2_conv_all_nth)
+
+lemma ex_not: "((\<forall>x. P x) \<longrightarrow> False) = (\<exists>x. \<not>P x)"
+  by simp
+
+lemma "nonrep_list ([1, 1, 1]::nat list) \<longrightarrow> False"
+  apply (unfold nonrep_list_def eq_shape_list_def eq_shape_list_alt)
+  apply (rule ex_not[THEN iffD2])
+  apply (rule exI[of _ "[1, 2, 3]"])
+  apply (auto)
+  done
+
+lemma "nonrep_list ([1, 2, 3]::nat list)"
+  apply (unfold nonrep_list_def eq_shape_list_def eq_shape_list_alt)
+  apply (rule allI)
+  apply (rule impI)
+  subgoal for x
+    apply (rule exI[of _ "(\<lambda> y. (if y = 1 then (hd x) else (if y = 2 then (hd (tl x)) else (hd (tl (tl x))))))"])
+    apply (auto)
+    by (metis (lifting) ext length_0_conv length_Suc_conv list.sel(1,3))
+  done
+
+typedef 'a nrp_list = "{(xs :: 'a list). nonrep_list xs}"
+  apply (rule exI[of _ "[]"])
+  apply (auto simp add: nonrep_list_def eq_shape_list_def)
+  done
+
+(* PROD *)
+definition eq_shape_prod_1 :: "('a \<times> 'b) \<Rightarrow> ('a \<times> 'b) \<Rightarrow> bool" where 
+  "eq_shape_prod_1 x x' \<equiv> rel_prod top (=) x x'"
+
+definition nonrep_prod_1 :: "('a \<times> 'b) \<Rightarrow> bool" where 
+  "nonrep_prod_1 x \<equiv> \<forall> x'. eq_shape_prod_1 x x' \<longrightarrow> (\<exists> f. x' = map_prod f id x)"
+
+(* any product is nonrep on first position*)
+lemma "nonrep_prod_1 (a, b)"
+  apply (unfold nonrep_prod_1_def eq_shape_prod_1_def)
+  apply (auto)
+  done
+
+section "Intuition: What is strong pullback perservation?"
+(* fset *)
+lemma "rel_fset top (Abs_fset {1, 2}) (Abs_fset {1, 2})"
+  unfolding fset.in_rel[unfolded mem_Collect_eq] 
+  apply (rule exI[of _ "(Abs_fset {(1, 2), (2, 1)})"], auto)
+  apply (subst Abs_fset_inverse[unfolded mem_Collect_eq], simp,
+    subst (asm) Abs_fset_inverse[unfolded mem_Collect_eq], auto)+
+  done
+
+lemma "rel_fset top (Abs_fset {1, 2}) (Abs_fset {1, 2})"
+  unfolding fset.in_rel[unfolded mem_Collect_eq] 
+  apply (rule exI[of _ "(Abs_fset {(1, 1), (2, 2)})"], auto)
+  apply (subst Abs_fset_inverse[unfolded mem_Collect_eq], simp,
+    subst (asm) Abs_fset_inverse[unfolded mem_Collect_eq], auto)+
+  done
+ (* \<Longrightarrow> NOT \<exists>!z *)
+
+(* uprod *)
+lemma "rel_uprod top (Upair 1 2) (Upair 1 2)"
+  unfolding uprod.in_rel[unfolded mem_Collect_eq]
+  by (rule exI[of _ "Upair (1, 1) (2, 2)"]) auto
+
+lemma "rel_uprod top (Upair 1 2) (Upair 1 2)"
+  unfolding uprod.in_rel[unfolded mem_Collect_eq]
+  by (rule exI[of _ "Upair (1, 2) (2, 1)"]) auto
+ (* \<Longrightarrow> NOT \<exists>!z *)
+
+section "Intuition: Why BNF?"
+
+typedef 'a even_list = "{x :: 'a list. even (length x)}"
+  apply (rule exI[of _ "[]"])
+  apply (unfold mem_Collect_eq list.size(3))
+  apply (rule even_zero)
+  done
+
+datatype 'a test_A = F 'a | R "('a test_A) set"
+datatype 'a test_B = MK "'a" | MK2 "('a test_B) even_list"
+
+setup_lifting type_definition_even_list
+lift_bnf 'a even_list [wits: "[] :: 'a list"] 
+  subgoal for f x
+    apply (unfold mem_Collect_eq length_map)
+    apply (assumption)
+    done
+  subgoal for z
+    apply (unfold mem_Collect_eq)
+    apply (intro bexI[of _ z] conjI subset_refl refl)
+    apply (unfold mem_Collect_eq length_map)
+    apply (assumption)
+    done
+  subgoal
+  apply (unfold mem_Collect_eq list.size(3))
+  apply (rule even_zero)
+    done
+  subgoal for a
+    apply (unfold list.set(1) empty_iff)
+    apply (assumption)
+    done
+  done
+
+thm fun.set_bd
+(*
+bnf "'a set"
+  map: image
+    sets: "(id :: 'a set \<Rightarrow> 'a set)"
+  bd: "natLeq +c card_suc |UNIV|"
+  rel: rel_set
+           apply (auto simp add: card_order_bd_fun Cinfinite_bd_fun[THEN conjunct1] regularCard_bd_fun)
+  subgoal for f g
+    by fastforce
+  subgoal for x
+    using card_of_UNIV ordLeq_ordLess_trans ordLess_bd_fun by blast
+  subgoal for R S x y z
+    apply (unfold rel_set_def)
+    by (meson relcomppI)
+  apply (intro ext)
+  subgoal for R x y
+    sorry
+  done
+print_theorems
+*)
+
+
+datatype 'a test_A = F 'a | R "('a test_A) set" (* is set a BNF?*)
+datatype 'a test_B = MK "'a" | MK2 "('a test_B) even_list"
+
+
+linearize_mrbnf 'a::var lin_fset = "'a::var fset" on 'a
+  done
+
+binder_datatype 'a test_C = Leaf | MK2' "(r::'a) lin_fset" "s::'a test_C" binds r in s
+
+
+section "Example: Foo"
+setup \<open>Sign.qualified_path false (Binding.name "foo")\<close>
+
+codatatype ('a, 'b) foo = Foo "'a" | Bar 'b "('a, 'b) foo"
+
+setup \<open>Sign.parent_path\<close>
+
+mrbnf "('a, 'b) foo"
+  map: map_foo
+  sets: live: set1_foo live: set2_foo
+  bd: "card_suc natLeq"
+  wits:
+    "wit1_foo" "wit2_foo"
+  sorry
+
+print_mrbnfs
+
+primcorec mywit where
+  "mywit X = (let y = SOME x. x\<notin>X in Bar y (mywit (insert y X)))"
+
+linearize_mrbnf ('a, 'b::var_foo) foo'' = "('a, 'b::var_foo) foo" 
+  [wits: "(mywit {}) :: ('a, 'b::var_foo) foo"] on 'b
+  subgoal
+    sorry
+  subgoal
+    sorry
+  subgoal
+    sorry
+  done
+
+section "declaration: L, F, G"
+
+subsection "L"
+typedecl ('a, 'b) L
+consts map_L :: "('a \<Rightarrow> 'a') \<Rightarrow> ('b \<Rightarrow> 'b') \<Rightarrow> ('a, 'b) L \<Rightarrow> ('a', 'b') L"
+consts set1_L :: "('a, 'b) L \<Rightarrow> 'a set"
+consts set2_L :: "('a, 'b) L \<Rightarrow> 'b set"
+consts rrel_L :: "('a \<Rightarrow> 'a' \<Rightarrow> bool) \<Rightarrow> ('b \<Rightarrow> 'b' \<Rightarrow> bool) \<Rightarrow> ('a, 'b) L \<Rightarrow> ('a', 'b') L \<Rightarrow> bool"
+
+mrbnf "('a, 'b) L"
+  map: map_L
+  sets: live: set1_L live: set2_L
+  bd: natLeq
+  rel: rrel_L
+  var_class: var
+  sorry
+
+consts witL :: "('a::var, 'b) L"
+
+
+subsection "F"
+typedecl ('a, 'b, 'c, 'd, 'e, 'f) F
+consts map_F :: "('a \<Rightarrow> 'a') \<Rightarrow> ('b :: var \<Rightarrow> 'b) \<Rightarrow>
+  ('c :: var \<Rightarrow> 'c) \<Rightarrow> ('e \<Rightarrow> 'e') \<Rightarrow> ('f \<Rightarrow> 'f') \<Rightarrow> ('a, 'b, 'c, 'd, 'e, 'f) F \<Rightarrow> ('a', 'b, 'c, 'd, 'e', 'f') F"
+consts set1_F :: "('a, 'b :: var, 'c :: var, 'd, 'e, 'f) F \<Rightarrow> 'a set"
+consts set2_F :: "('a, 'b :: var, 'c :: var, 'd, 'e, 'f) F \<Rightarrow> 'b set"
+consts set3_F :: "('a, 'b :: var, 'c :: var, 'd, 'e, 'f) F \<Rightarrow> 'c set"
+consts set4_F :: "('a, 'b :: var, 'c :: var, 'd, 'e, 'f) F \<Rightarrow> 'e set"
+consts set5_F :: "('a, 'b :: var, 'c :: var, 'd, 'e, 'f) F \<Rightarrow> 'f set"
+consts rrel_F :: "('a \<Rightarrow> 'a' \<Rightarrow> bool) \<Rightarrow> ('e \<Rightarrow> 'e' \<Rightarrow> bool) \<Rightarrow> ('f \<Rightarrow> 'f' \<Rightarrow> bool) \<Rightarrow> ('a, 'b :: var, 'c :: var, 'd, 'e, 'f) F \<Rightarrow> ('a', 'b, 'c, 'd, 'e', 'f') F \<Rightarrow> bool"
+
+mrbnf "('a, 'b :: var, 'c :: var, 'd, 'e, 'f) F"
+  map: map_F
+  sets: live: set1_F bound: set2_F free: set3_F live: set4_F live: set5_F 
+  bd: natLeq
+  rel: rrel_F
+  var_class: var
+  sorry
+
+subsection "G"
+typedecl ('a, 'b, 'c, 'd, 'e, 'f) G
+consts map_G :: "('a \<Rightarrow> 'a') \<Rightarrow> ('b \<Rightarrow> 'b') \<Rightarrow>
+  ('c \<Rightarrow> 'c') \<Rightarrow> ('d \<Rightarrow> 'd') \<Rightarrow> ('e  \<Rightarrow> 'e') \<Rightarrow> ('a, 'b, 'c, 'd, 'e, 'f) G \<Rightarrow> ('a', 'b', 'c', 'd', 'e', 'f) G"
+consts set1_G :: "('a, 'b , 'c , 'd, 'e , 'f) G \<Rightarrow> 'a set"
+consts set2_G :: "('a, 'b , 'c , 'd, 'e , 'f) G \<Rightarrow> 'b set"
+consts set3_G :: "('a, 'b , 'c , 'd, 'e , 'f) G \<Rightarrow> 'c set"
+consts set4_G :: "('a, 'b , 'c , 'd, 'e , 'f) G \<Rightarrow> 'd set"
+consts set5_G :: "('a, 'b , 'c , 'd, 'e , 'f) G \<Rightarrow> 'e set"
+consts rrel_G :: "('a \<Rightarrow> 'a' \<Rightarrow> bool) \<Rightarrow> ('b \<Rightarrow> 'b' \<Rightarrow> bool) \<Rightarrow> ('c \<Rightarrow> 'c' \<Rightarrow> bool) \<Rightarrow> 
+  ('d \<Rightarrow> 'd' \<Rightarrow> bool) \<Rightarrow> ('e \<Rightarrow> 'e' \<Rightarrow> bool) \<Rightarrow> ('a, 'b , 'c , 'd, 'e, 'f) G \<Rightarrow> ('a', 'b', 'c', 'd', 'e', 'f) G \<Rightarrow> bool"
+consts wit1_G :: "'a \<Rightarrow> 'b \<Rightarrow> ('a, 'b, 'c, 'd, 'e, 'f) G"
+consts wit2_G :: "'c \<Rightarrow> 'd \<Rightarrow> ('a, 'b, 'c, 'd, 'e, 'f) G"
+consts wit3_G :: "'b \<Rightarrow> 'e \<Rightarrow> ('a, 'b, 'c, 'd, 'e, 'f) G"
+
+mrbnf "('a, 'b, 'c, 'd, 'e, 'f) G" 
+  map: map_G
+  sets: live: set1_G live: set2_G live: set3_G live: set4_G live: set5_G
+  bd: natLeq
+  wits:
+    "wit1_G :: 'a \<Rightarrow> 'b \<Rightarrow> ('a, 'b, 'c, 'd, 'e, 'f) G"
+    "wit2_G :: 'c \<Rightarrow> 'd \<Rightarrow> ('a, 'b, 'c, 'd, 'e, 'f) G"
+    "wit3_G :: 'b \<Rightarrow> 'e \<Rightarrow> ('a, 'b, 'c, 'd, 'e, 'f) G"
+  rel: rrel_G
+  var_class: var
+  sorry
+
+consts wit1_lG :: "'a \<Rightarrow> 'b \<Rightarrow> ('a, 'b, 'c, 'd, 'e, 'f) G" 
+consts wit2_lG :: "'a \<Rightarrow> ('a, 'b, 'c, 'd, 'e, 'f) G"
+consts wit3_lG :: "('a, 'b, 'c, 'd, 'e, 'f) G"
+consts wit4_lG :: "'c \<Rightarrow> ('a, 'b, 'c, 'd, 'e, 'f) G"
+
+
+section "linearize"
+
+subsection "L"
+linearize_mrbnf ('a::var, 'b) L' = "('a::var, 'b) L" [wits:"witL :: ('a::var, 'b) L"] on 'a
+  sorry
+
+linearize_mrbnf ('a, 'b::var) L'' = "('a, 'b::var) L" on 'b 
+  for eq_shape: sm_shp_L2 nonrep: nrp_shp_L2
+  sorry
+
+subsection "F"
+linearize_mrbnf ('a, 'b::var, 'c::var, 'd, 'e::var, 'f::var) F'' = "('a, 'b::var, 'c::var, 'd, 'e::var, 'f::var) F" on 'f and 'e
+  sorry
+
+linearize_mrbnf (st1:'b::var, st2:'f , st3:'c::var , 'd, st4:'a::var , st5:'e) F''' = 
+  "('a::var, 'b::var, 'c::var, 'd, 'e, 'f) F" on 'a for eq_shape: sm_shp_F3 nonrep: nrp_shp_F3
+  sorry
+
+subsection "G"
+linearize_mrbnf ('a, 'b, 'c::var, 'd::var, 'e, 'f) lG = "('a, 'b, 'c::var, 'd::var, 'e, 'f) G" 
+  [wits:"wit1_lG :: 'a \<Rightarrow> 'b \<Rightarrow> ('a, 'b, 'c::var, 'd::var, 'e, 'f) G" 
+    (*"wit2_lG :: 'a \<Rightarrow> ('a, 'b, 'c::var, 'd::var, 'e, 'f) G"*)
+    (*"wit3_lG :: ('a, 'b, 'c::var, 'd::var, 'e, 'f) G"*)] on 'd and 'c
+  sorry
+
+lemma nonrep_G_wit1: "nonrep_G (wit1_G a b)"
+  apply (unfold nonrep_G_def eq_shape_G_def mr_rel_G_def G.in_rel mem_Collect_eq)
+  apply (intro allI impI)
+  apply (erule exE)
+  apply (rule exI[of _ id])
+  apply (rule exI[of _ id])
+  apply (subst G.map_id)
+  apply (elim conjE)
+  apply (hypsubst_thin)
+  apply (unfold triv_forall_equality) (*?*)
+  apply (rule trans[OF sym, rotated])
+   apply assumption
+  apply (rule G.map_cong; (rule refl)?)
+      apply (unfold split_paired_all fst_conv snd_conv)
+      defer 3 (* lin_pos - idx *)
+      defer 3
+      apply (drule rev_subsetD, 
+      assumption, 
+      drule Set.CollectD, 
+      subst (asm) case_prod_conv, 
+      assumption)+
+
+  apply (drule arg_cong[of _ _ set3_G])
+  apply (subst (asm) G.set_map)
+  apply (subst (asm) set_eq_iff)
+  apply (subst (asm) image_iff)
+  apply (drule spec)
+  apply (drule iffD1)
+   apply (rule bexI[rotated])
+    apply assumption
+    apply (rule fst_conv[symmetric])
+  apply (drule G.wit1)
+   apply (erule FalseE)
+
+  apply (drule arg_cong[of _ _ set4_G])
+  apply (subst (asm) G.set_map)
+  apply (subst (asm) set_eq_iff)
+  apply (subst (asm) image_iff)
+  apply (drule spec)
+  apply (drule iffD1)
+   apply (rule bexI[rotated])
+    apply assumption
+   apply (rule fst_conv[symmetric])
+  apply (drule G.wit1)
+  apply (erule FalseE)
+  done
+
+
+lemma "x \<in> set1_lG (Abs_lG (wit1_G a b)) \<Longrightarrow> x = a"
+      "x \<in> set2_lG (Abs_lG (wit1_G a b)) \<Longrightarrow> x = b"
+      "x \<in> set3_lG (Abs_lG (wit1_G a b)) \<Longrightarrow> False"
+      "x \<in> set4_lG (Abs_lG (wit1_G a b)) \<Longrightarrow> False"
+     apply (unfold set1_lG_def set2_lG_def set3_lG_def set4_lG_def o_apply)
+  apply (unfold Abs_lG_inverse[unfolded mem_Collect_eq, OF nonrep_G_wit1])
+  apply (erule G.wit1)+
+  done
+
+
+subsection "other"
+linearize_mrbnf 'a :: var distinct_list = "('a ::var) list" on 'a
+  done
+
+linearize_mrbnf ('a::var, 'b) pair = "('a \<times> 'b) \<times> ('a::var)" on 'a
+  sorry
+end
